Primitive_Matchers/IpAddresses_Normalize.thy
@@ -130,7 +130,9 @@ text{*unused*}
   fun ipt_ipv4range_invert :: "ipt_ipv4range \<Rightarrow> (ipv4addr \<times> nat) list" where
     "ipt_ipv4range_invert (Ip4Addr addr) = ipv4range_split (wordinterval_invert (ipv4range_single (ipv4addr_of_dotdecimal addr)))" | 
     "ipt_ipv4range_invert (Ip4AddrNetmask base len) = ipv4range_split (wordinterval_invert 
-        (prefix_to_range (ipv4addr_of_dotdecimal base AND NOT mask (32 - len), len)))"
+        (prefix_to_range (ipv4addr_of_dotdecimal base AND NOT mask (32 - len), len)))" | 
+    "ipt_ipv4range_invert (Ip4AddrRange ip1 ip2) = ipv4range_split (wordinterval_invert
+      (ipv4range_range (ipv4addr_of_dotdecimal ip1, ipv4addr_of_dotdecimal ip2)))"
 
       
 
@@ -143,8 +145,48 @@ text{*unused*}
     done
 
 
-  
-  lemma ipt_ipv4range_invert_case_Ip4AddrNetmask:
+  (*this should be the generic case we need to show*)
+  lemma ipt_ipv4range_invert_case_Ip4AddrRange:
+      "(\<Union> ((\<lambda> (base, len). ipv4range_set_from_bitmask base len) ` (set (ipt_ipv4range_invert (Ip4AddrRange ip1 ip2))) )) = 
+        - {ipv4addr_of_dotdecimal ip1 ..  ipv4addr_of_dotdecimal ip2}"
+     proof - 
+      { fix r
+        have "\<forall>pfx\<in>set (ipv4range_split (wordinterval_invert r)). valid_prefix pfx" using all_valid_Ball by blast
+        with prefix_bitrang_list_union have
+        "\<Union>((\<lambda>(base, len). ipv4range_set_from_bitmask base len) ` set (ipv4range_split (wordinterval_invert r))) =
+        wordinterval_to_set (list_to_wordinterval (map prefix_to_range (ipv4range_split (wordinterval_invert r))))" by simp
+        also have "\<dots> = wordinterval_to_set (wordinterval_invert r)"
+          unfolding wordinterval_eq_set_eq[symmetric] using ipv4range_split_union[of "(wordinterval_invert r)"] ipv4range_eq_def by simp
+        also have "\<dots> = - wordinterval_to_set r" by auto
+        finally have "\<Union>((\<lambda>(base, len). ipv4range_set_from_bitmask base len) ` set (ipv4range_split (wordinterval_invert r))) = - wordinterval_to_set r" .
+      } from this[of "(ipv4range_range (ipv4addr_of_dotdecimal ip1, ipv4addr_of_dotdecimal ip2))"]
+        show ?thesis
+        apply(simp only: ipt_ipv4range_invert.simps)
+        apply(simp add: prefix_to_range_set_eq)
+        apply(simp add: ipv4range_range.simps)
+        done
+     qed
+
+
+  lemma prefix_to_range_eq_ipv4range_range: "(prefix_to_range (addr, len)) = (ipv4range_range (addr, (addr || pfxm_mask (addr, len))))"
+    apply(simp add: ipv4range_range.simps)
+    apply(simp add: pfxm_mask_def pfxm_length_def)
+    apply(simp add: prefix_to_range_def)
+    apply(simp add: pfxm_prefix_def pfxm_mask_def pfxm_length_def)
+    done
+
+  (* okay, we only need to focus in the generic case *)
+  lemma ipt_ipv4range_invert_case_Ip4AddrNetmask: "ipt_ipv4range_invert (Ip4AddrNetmask addr len) =
+        ipt_ipv4range_invert (Ip4AddrRange
+          (dotdecimal_of_ipv4addr (ipv4addr_of_dotdecimal addr && ~~ mask (32 - len)))
+          (dotdecimal_of_ipv4addr (ipv4addr_of_dotdecimal addr && ~~ mask (32 - len) || pfxm_mask (ipv4addr_of_dotdecimal addr && ~~ mask (32 - len), len))))"
+    apply(simp)
+    apply(simp add: prefix_to_range_eq_ipv4range_range)
+    apply(simp add: ipv4range_range.simps)
+    apply(simp add: ipv4addr_of_dotdecimal_dotdecimal_of_ipv4addr)
+    done
+
+  (*lemma ipt_ipv4range_invert_case_Ip4AddrNetmask:
       "(\<Union> ((\<lambda> (base, len). ipv4range_set_from_bitmask base len) ` (set (ipt_ipv4range_invert (Ip4AddrNetmask base len))) )) = 
         - (ipv4range_set_from_bitmask (ipv4addr_of_dotdecimal base) len)"
      proof - 
@@ -164,16 +206,25 @@ text{*unused*}
         apply(simp add: cornys_hacky_call_to_prefix_to_range_to_start_with_a_valid_prefix pfxm_length_def pfxm_prefix_def wordinterval_to_set_ipv4range_set_from_bitmask)
         (*apply(thin_tac "?X")*)
         by (metis ipv4range_set_from_bitmask_alt1 ipv4range_set_from_netmask_base_mask_consume maskshift_eq_not_mask)
-     qed
+     qed *)
 
   lemma ipt_ipv4range_invert: "(\<Union> ((\<lambda> (base, len). ipv4range_set_from_bitmask base len) ` (set (ipt_ipv4range_invert ips)) )) = - ipv4s_to_set ips"
     apply(cases ips)
-     apply(simp_all only:)
-     prefer 2
-     using ipt_ipv4range_invert_case_Ip4AddrNetmask apply simp
-    apply(subst ipt_ipv4range_invert_case_Ip4Addr) (* yayyy, do the same proof again *)
-    apply(subst ipt_ipv4range_invert_case_Ip4AddrNetmask)
-    apply(simp add: ipv4range_set_from_bitmask_32)
+      apply(simp_all only:)
+      prefer 3
+      apply(subst ipt_ipv4range_invert_case_Ip4AddrRange)
+      apply(simp; fail)
+     apply(simp_all only: ipt_ipv4range_invert_case_Ip4AddrNetmask ipt_ipv4range_invert_case_Ip4Addr) (*yay, do the same proof again and again*)
+     apply(subst ipt_ipv4range_invert_case_Ip4AddrRange)
+     apply(simp)
+     apply(simp add: ipv4addr_of_dotdecimal_dotdecimal_of_ipv4addr)
+     apply(simp add: pfxm_mask_def pfxm_length_def)
+    apply(subst ipt_ipv4range_invert_case_Ip4AddrRange)
+    apply(simp)
+    apply(simp add: ipv4addr_of_dotdecimal_dotdecimal_of_ipv4addr)
+    apply(simp add: pfxm_mask_def pfxm_length_def)
+    apply(simp add: ipv4range_set_from_bitmask_alt maskshift_eq_not_mask) (*sledgehammer here uses more than 8GB ram*)
+    apply(simp add: maskshift_eq_not_mask word_bw_comms(2) word_oa_dist2)
     done
 
  
